src/fstar/FStarC.CheckedFiles.fsti
@@ -60,6 +60,10 @@ val load_parsing_data_from_cache: file_name:string -> option Parser.Dep.parsing_
 (* Loading and storing cache files                                     *)
 (***********************************************************************)
 
+//checks if the cache files exists and all their dependences are valid
+//returning the names of all the dependences if so
+val scan_deps_and_check_cache_validity (_:Dep.deps) (file:string) : option (list string & Dep.deps)
+
 val load_module_from_cache: TcEnv.env -> string -> option tc_result
 
 val store_module_to_cache: TcEnv.env -> file_name:string -> (Dep.parsing_data & list string) -> tc_result -> unit
